tests/lean/run/cases_term.lean
@@ -1,0 +1,10 @@
+example (f : nat → nat) (p : nat → Prop)
+        (h₁ : ∀ x, f (nat.succ x) = 1)
+        (h₂ : ¬ p 0)
+        (a : nat)
+        (h₃ : p (f a)) : f (f a) = 1 :=
+begin
+  cases f a,
+  contradiction,
+  apply h₁
+end
